

Bilinear form:

Defn (Bilinear form): V n -dim'l vector space over \mathbb{R} , \langle, \rangle is a bilinear form if

$$\langle, \rangle : V \times V \rightarrow \mathbb{R}.$$

$$(v, w) \mapsto \langle v, w \rangle.$$

$$a \in \mathbb{R}, v, w \in V. \quad v_1, v_2 \in V.$$

$$\textcircled{1} \quad \langle av, w \rangle = a \langle v, w \rangle$$

$$\langle v_1 + v_2, w \rangle = \langle v_1, w \rangle + \langle v_2, w \rangle$$

$$\textcircled{2} \quad \langle w, av \rangle = a \langle w, v \rangle$$

$$\langle w, v_1 + v_2 \rangle = \langle w, v_1 \rangle + \langle w, v_2 \rangle.$$

Defn (Symmetric bilinear form) or symmetric form

$$\langle v, w \rangle = \langle w, v \rangle$$

Defn (Skew symmetric form, alternating form)

$$\langle v, w \rangle = - \langle w, v \rangle$$

Ex 1: Euclidean space $\mathbb{R}^n = \left\{ \begin{pmatrix} x_1 \\ \vdots \\ x_n \end{pmatrix} \right\}$

$$v = \begin{pmatrix} x_1 \\ \vdots \\ x_n \end{pmatrix}, \quad w = \begin{pmatrix} y_1 \\ \vdots \\ y_n \end{pmatrix}$$

$$\langle v, w \rangle = \sum x_i y_i. \quad (\text{standard inner product})$$

Angle between non zero v, w ,

$$\cos \theta = \frac{\langle v, w \rangle}{\sqrt{\langle v, v \rangle \langle w, w \rangle}}$$

Ex 2: Minkowski space. (Lorentz form)

$$\langle v, w \rangle = x_1 y_1 + x_2 y_2 \dots x_{n-1} y_{n-1} - x_n y_n.$$

Ex 1, Ex 2 are symmetric bilinear forms.

Gram matrix $B: v_1, \dots, v_n$ basis of V . \langle, \rangle bilinear

$$(\langle v_i, v_j \rangle)_{n \times n} = G_{B, \langle, \rangle}$$

$$\forall v \in V, \quad v = \sum_{i=1}^n x_i v_i, \quad w = \sum_{j=1}^n y_j v_j$$

$$x = \begin{pmatrix} x_1 \\ \vdots \\ x_n \end{pmatrix} = (\bar{v})_B, \quad y = \begin{pmatrix} y_1 \\ \vdots \\ y_n \end{pmatrix} = (\bar{w})_B$$

$$\text{Prop: } \langle v, w \rangle = x^T \cdot G_{B, \langle, \rangle} y$$

$$\text{Prop: If } (w_1, \dots, w_n) = (v_1, \dots, v_n) \cdot P$$

is another basis, then

Gram matrix under basis $B': (w_1, \dots, w_n)$

$$G_{\langle, \rangle, B'} = P^T G_{\langle, \rangle, B} P \quad (\Leftarrow \text{matrix congruence})$$

$$\text{Pf: } P = (p_{ij}), \quad w_j = \sum_i p_{ij} v_i$$

$$\langle w_j, w_k \rangle = \langle \sum_i p_{ij} v_i, \sum_l p_{lk} v_l \rangle$$

$$\Rightarrow G_{\langle, \rangle, B'} = P^T G_{\langle, \rangle, B} P$$

$\forall f_h: A_1, A_2 \in M_n(\mathbb{R})$, congruent iff $\exists P \in GL(n, \mathbb{R})$

$$\text{s.t. } P^T A_1 P = A_2 \quad (\text{相合})$$

Defn: (Isometry) $(V_1, \langle \cdot, \cdot \rangle_1), (V_2, \langle \cdot, \cdot \rangle_2)$

isometric iff $\exists f: V_1 \rightarrow V_2$ s.t.

$$\langle v, w \rangle_1 = \langle f(v), f(w) \rangle_2 \quad \forall v, w \in V_1$$

(Such an f is called isometry)

Prop: $(V_1, \langle \cdot, \cdot \rangle_1), (V_2, \langle \cdot, \cdot \rangle_2)$

are isometric iff the two Gram matrices are congruent.

Ex: $V = M_{m \times n}(\mathbb{R})$, $\langle \cdot, \cdot \rangle_F$ (Frobenius)

$$\langle A, B \rangle_F = \text{Tr}(A^T B)$$

$V, \langle \cdot, \cdot \rangle_F$ isometric to \mathbb{R}^{mn} , $\langle \cdot, \cdot \rangle_{\text{standard}}$

Prop: $V, \langle \rangle$ symmetric iff the Gram matrices are symmetric ($A = A^T$)

From now on: \langle, \rangle is symmetric.

Prop: (polarization identity) \langle, \rangle symmetric, then

$$\langle v, w \rangle = \frac{1}{2} (\langle v+w, v+w \rangle - \langle v, v \rangle - \langle w, w \rangle)$$

Pf: By expansion.

Thm: There exists basis of V , v_1, \dots, v_n , (Sylvester) such that $v = \sum x_i v_i$.

$$\langle v, v \rangle = x_1^2 + \dots + x_p^2 - x_{p+1}^2 - \dots - x_{p+q}^2$$

p, q are determined by \langle, \rangle .

... uniqueness

or

$$G_{\langle, \rangle} B = \begin{bmatrix} I_p & & \\ & -I_q & \\ & & 0 \end{bmatrix}$$

Pf: (Existence)

By polarization identity, if $\langle \cdot, \cdot \rangle$ is not zero,
then $\exists v_1 \in V$, s.t. $\langle v_1, v_1 \rangle = a \neq 0$.

Define $W = \{ w \in V \mid \langle w, v_1 \rangle = 0 \}$.

Claim: $W \oplus \mathbb{R}v_1 = V$.

(a) $W \cap \mathbb{R}v_1 = \{0\}$. If $c v_1 \in W$.
 $\langle c v_1, v_1 \rangle = ca = 0 \Rightarrow c = 0$

(b) $\forall v \in V$, (Try to find c , s.t.

$$v = w + c v_1, \quad w \in W$$

$$\Leftrightarrow \langle v - c v_1, v_1 \rangle = 0$$

$$\Leftrightarrow c = \frac{\langle v, v_1 \rangle}{\langle v_1, v_1 \rangle}$$

$$\text{Let } c = \frac{\langle v, v_1 \rangle}{\langle v_1, v_1 \rangle}$$

Then $v - c v_1 = w \in W \Rightarrow v \in W + \mathbb{R}v_1$

$\dim W = n-1$, By induction on n .

W has basis w_1, \dots, w_{n-1} s.t.

$$\langle w_i, w_j \rangle = \begin{cases} 0 & i \neq j \\ \pm 1, 0 & i = j \end{cases}$$

$$\text{Let } w_0 = \frac{v_1}{\sqrt{|a|}} \Rightarrow \langle w_0, w_i \rangle = 0 \quad \forall i \geq 0$$
$$\langle w_0, w_0 \rangle = \pm 1.$$

Rearrange the order of $w_0, \dots, w_{n-1} \Rightarrow$

Basis v_1, \dots, v_n s.t. $\langle v_i, v_j \rangle$

$$= \begin{cases} 0 & i \neq j \\ 1 & 1 \leq i \leq j \leq p \\ -1 & p+1 \leq i \leq j \leq p+q \\ 0 & i \neq j \geq p+q+1 \end{cases}$$

(The same method for any field \Rightarrow Basis s.t. Gram matrix is diagonal)

Uniqueness:

$$W_1 = \text{span}(v_1, \dots, v_p)$$

$$W_2 = \text{span}(v_{p+1}, \dots, v_{p+q})$$

$$W_3 = \text{span}(v_{p+q+1}, \dots, v_n)$$

$$V = W_1 \oplus W_2 \oplus W_3$$

If under basis $B' : v_1' \dots v_{p'}' \dots$
 $v_{q'}' \dots v_n'$ s.t. $\{v_i' \mid i \in I\} =$

$$\begin{bmatrix} I_{p'} \\ & -I_{q'} \\ & & 0 \end{bmatrix}$$

then $V = W_1' \oplus W_2' \oplus W_3'$, and we claim

$$\dim W_i = \dim W_i',$$

If $\dim W_1 > \dim W_1'$, then $\dim W_1 + \dim(W_2' \oplus W_3') > n$

$$\Rightarrow W_1 \cap (W_2' \oplus W_3') \neq 0.$$

$$\Rightarrow \exists v = \sum_{i=1}^p a_i v_i = \sum_{j=p'+1}^n b_j' v_j' \neq 0,$$

$$\Rightarrow \langle v, v \rangle = \sum_{i=1}^p a_i^2 > 0 \quad (\text{since not all } a_i = 0)$$

$$\langle v, v \rangle = -\sum_{j=p'+1}^{p'+q'} b_j'^2 \leq 0. \quad \text{Contradiction}$$

$$\text{So } \dim W_1 \leq \dim W_1'$$

For the same reason $\dim W_1 \geq \dim W_1'$

$$p = p', \quad \text{and} \quad q = q'. \quad \Rightarrow (p, q, n-p-q)$$

$$= (p', q', n-p'-q') \quad \square$$

$(p, q, n-p-q)$ is called the signature of \langle, \rangle .

Sylvester Thm in terms of matrices:

Thm: For any symmetric ^{real} matrix A ,

$\exists P$ invertible, s.t.

$$P^T A P = \begin{pmatrix} I_p & & \\ & -I_q & \\ & & 0 \end{pmatrix}$$

and $(p, q, n-p-q)$ uniquely determines the congruence class of A .

(signature of A)